\begin{pr}$ $
\begin{enumerate}[(a)]
\item $A$ and $B$ are independent $\iff\P[A\cap B]=\P[A]\P[B]\iff\P[A\cap B^c]\overtext{proved in problem 3}=\P[A]-\P[A\cap B]=\P[A]-\P[A]\P[B]=\P[A](1-\P[B])=\P[A]\P[B^c]\iff A$ and $B^c$ are independent.
\item $A$ and $B$ are independent $\iff\P[A\cap B]=\P[A]\P[B]\iff\P[A^c\cap B]\overtext{proved in problem 3}=\P[B]-\P[A\cap B]=\P[B]-\P[A]\P[B]=\P[B](1-\P[A])=\P[B]\P[A^c]\iff A^c$ and $B$ are independent.
\item From (b), $A$ and $B$ are independent $\iff A^c$ and $B$ are independent $\iff\P[A^c\cap B]=\P[A^c]\P[B]\iff\P[A^c\cap B^c]\overtext{proved in problem 3}=\P[A^c]-\P[A^c\cap B]=\P[A^c]-\P[A^c]\P[B]=\P[A^c](1-\P[B])=\P[A^c]\P[B^c]\iff A^c$ and $B^c$ are independent.
\end{enumerate}
\end{pr}
