\begin{pr}
First, there are two lemmas:

\begin{lm}\label{not}
$E\subseteq F\iff\sim F\subseteq\sim E$.
\end{lm}

\begin{lm}\label{pk}
$PE=\sim K\sim E$.
\end{lm}

Let's prove P2, P4 by K2, K4.\\
$K\sim E\overtext{K2}\subseteq\sim E\overtext{\rflm{not}}\then E\subseteq\sim K\sim E\overtext{\rflm{pk}}=PE$, which is P2.\\
$P\sim E\overtext{K4}\subseteq KP\sim E\overtext{\rflm{not}}\then PKE\overtext{\rflm{pk}}=P\sim P\sim E\overtext{\rflm{pk}}=\sim KP\sim E\subseteq\sim P\sim E\overtext{\rflm{pk}}=KE$, which is P4.\\
$KE\overtext{P2}\subseteq PKE\overtext{K4}\subseteq KPKE\overtext{P4}\subseteq K^2E$.
\end{pr}
