\begin{pr}$ $
\begin{enumerate}[(a)]
\item $\pi_0^{(n)}(x^n)=\P\{\Theta=0|X^n=x^n\}=\P\{X_i\overtext{i.i.d.}\sim P_0|X^n=x^n\}=\frac{\P\{X_i\overtext{i.i.d.}\sim P_0\land X^n=x^n\}}{\P\{X^n=x^n\}}=\frac{\P\{X_i\overtext{i.i.d.}\sim P_0\land X^n=x^n\}}{\P\{(X_i\overtext{i.i.d.}\sim P_0\land X^n=x^n)\lor(X_i\overtext{i.i.d.}\sim P_1\land X^n=x^n)\}}=\frac{\pi_0^{(0)}\prodl_{i=1}^nP_0(x_i)}{\pi_0^{(0)}\prodl_{i=1}^nP_0(x_i)+\pi_1^{(0)}\prodl_{i=1}^nP_1(x_i)}$.\\
Similarly, $\pi_1^{(n)}(x^n)=\frac{\pi_1^{(0)}\prodl_{i=1}^nP_1(x_i)}{\pi_0^{(0)}\prodl_{i=1}^nP_0(x_i)+\pi_1^{(0)}\prodl_{i=1}^nP_1(x_i)}$.
\item $-\frac1n\log\pi_0^{(0)}\prodl_{i=1}^nP_0(X_i)=-\frac1n\left(\log\pi_0^{(0)}+\suml_{i=1}^n\log(P_0(X_i))\right)\overtext{SLLN}\to-\frac1n\log\pi_0^{(0)}-\E[\log(P_0(X))]\overset{\log\pi_0^{(0)}\text{ is a constant}}\to-\E[\log(P_0(X))]=H(X)$ as $n\to\infty$.\\
From HW2 we know that $H(X)\leq-\suml_{i=1}^\infty P_0(i)\log P_1(i)$, with equality $\iff P_1\sim P_0$.\\
$-\frac1n\log\pi_1^{(0)}\prodl_{i=1}^nP_1(X_i)=-\frac1n\left(\log\pi_1^{(0)}+\suml_{i=1}^n\log(P_1(X_i))\right)\overtext{SLLN}\to-\frac1n\log\pi_1^{(0)}-\E[\log(P_1(X))]\overset{\log\pi_1^{(0)}\text{ is a constant}}\to-\E[\log(P_1(X))]>H(X)$ as $n\to\infty$.\\
$\then\frac{\pi_1^{(0)}\prodl_{i=1}^nP_1(X_i)}{\pi_0^{(0)}\prodl_{i=1}^nP_0(X_i)}\to\exp_2(nE[\log(P_1(X))]+nH(X))=\exp_2(E[\log(P_1(X))]+H(X))^n\overset{\E[\log(P_1(X))]+H(X)<0}\to0$ as $n\to\infty$.\\
$\so\pi_0^{(n)}(X^n)=\frac{\pi_0^{(0)}\prodl_{i=1}^nP_0(x_i)}{\pi_0^{(0)}\prodl_{i=1}^nP_0(x_i)+\pi_1^{(0)}\prodl_{i=1}^nP_1(x_i)}=\frac1{1+\frac{\pi_1^{(0)}\prodl_{i=1}^nP_1(X_i)}{\pi_0^{(0)}\prodl_{i=1}^nP_0(X_i)}}\to\frac1{1+0}=1$ as $n\to\infty$.\\
As what we computed above, for any constant $c>0$, $-\frac1n\log\frac{\pi_1^{(0)}\prodl_{i=1}^nP_1(X_i)}{c\pi_0^{(0)}\prodl_{i=1}^nP_0(X_i)}\\
=H(X)+\E[\log(P_1(X))]+\frac1n\log c\overset{c\text{ is a constant}}\to H(X)+\E[\log(P_1(X))]=D(P_0\|P_1)$.\\
$\cuz\log$ is an increasing function, and $\frac{\pi_1^{(0)}\prodl_{i=1}^nP_1(X_i)}{\pi_0^{(0)}\prodl_{i=1}^nP_0(X_i)}<\frac{\pi_1^{(0)}\prodl_{i=1}^nP_1(X_i)}{\pi_0^{(0)}\prodl_{i=1}^nP_0(X_i)+\pi_1^{(0)}\prodl_{i=1}^nP_1(X_i)}\\
=\pi_1^{(n)}(X^n)<\frac{\pi_1^{(0)}\prodl_{i=1}^nP_1(X_i)}{2\pi_0^{(0)}\prodl_{i=1}^nP_0(X_i)}$ when $n\to\infty$.\\
$\so$ by squeeze theorem, $-\frac1n\log\pi_1^{(n)}(X^n)\to D(P_0\|P_1)$ as $n\to\infty$.
\end{enumerate}
\end{pr}
