\begin{pr}$ $
\begin{enumerate}[(a)]
\item Let $X\sim P$.\\
$\D(P\|G(p))=\suml_{x=1}^\infty P(x)\log\frac{P(x)}{Q(x)}=\suml_{x=1}^\infty P(x)\log\frac{P(x)}{(1-p)p^{x-1}}=\H(X)-\E[\log((1-p)p^{X-1})]=\H(X)-\log(1-p)-\E[(X-1)\log(p)]=H(X)-\log(1-p)-\log(p)E[X-1]=H(X)-\log(1-p)+\log p-\mu\log p$.\\
$\frac d{dp}\D(P\|G(p))=\frac1{1-p}+\frac1p-\frac1p\mu=\frac{1-(1-p)\mu}{p(1-p)}$, which equals to $0\iff\frac1{1-p}=\mu\iff p=1-\frac1\mu$.\\
One can also verify that if $p<1-\frac1\mu$, $\frac d{dp}\D(P\|G(p))<0$ and if $p>1-\frac1\mu$, $\frac d{dp}\D(P\|G(p))>0$.\\
$\so$ the minimum possible value of $\D(P\|G(p))$ occurs when $p=1-\frac1\mu$, that is, the distribution is $G(1-\frac1\mu)$, and $\D(P\|G(p))=H(X)-\log\mu+(1-\mu)\log(1-\mu)$.
\item Let $X_i\sim P_i, Y\sim R$ where $R(y):=\frac1m\suml_{i=1}^mP_i(y)$.\\
From HW2 we know that $H(R)\leq-\suml_{j=1}^\infty R(j)\log Q(j)$, with equality $\iff Q\sim R$.\\
$\then\suml_{i=1}^m\D(P_i\|Q)=\suml_{i=1}^m\left(H(X_i)-\suml_{j=1}^\infty P_i(j)\log Q(j)\right)=\suml_{i=1}^mH(X_i)-\suml_{j=1}^\infty\left(\suml_{i=1}^m P_i(j)\right)\log Q(j)=\suml_{i=1}^mH(X_i)-m\suml_{j=1}^\infty R(j)\log Q(j)\geq\suml_{i=1}^mH(X_i)-mH(R)$.\\
$\so\min_{Q\in\mathcal{P}(X)}\suml_{i=1}^mD(P_i\|Q)=\suml_{i=1}^mH(X_i)-mH(R)$, with minimizer $Q=R$, that is, $Q(y)=\frac 1m\suml_{i=1}^mP_i(y)$.
\end{enumerate}
\end{pr}
